Cube/Simple/Basic.lean
@@ -1,4 +1,7 @@
 import Cube.Util
+import Cube.Context
+
+import Mathlib.Tactic.Linarith
 
 import Lean
 
@@ -19,19 +22,18 @@ inductive Ast where
 
 inductive Expr where
 | bvar (idx : Nat)
-| fvar (name : String)
+| fvar (name : FVarId)
 | lam (ty : Ty) (body : Expr) (orig : String)
 | const (name : String)
 | app (func : Expr) (arg : Expr)
 deriving Repr, DecidableEq
-
 abbrev TranslationEnv := List String
 
 def Ast.toExpr : Ast → TranslationEnv → Expr
 | var name, vs =>
   match vs.findIdx? (name = ·) with
   | some idx => .bvar idx
-  | none => .fvar name
+  | none => .fvar ⟨name, 0⟩
 | const name, _ => .const name
 | app func arg, vs => .app (toExpr func vs) (toExpr arg vs)
 | lam x ty body, vs => .lam ty (toExpr body <| x :: vs) x
@@ -40,7 +42,7 @@ def Expr.toAst : Expr → TranslationEnv → Option Ast
 | bvar idx, vs => do
   let x ← vs[idx]?
   return .var x
-| fvar name, _ => some <| .var name
+| fvar fvarId, _ => some <| .var fvarId.name
 | lam ty body name, vs => do
     let body ← toAst body <| name :: vs
     return .lam name ty body
@@ -102,6 +104,158 @@ theorem Ast.toExpr_inv_toAst (a : Ast) (xs : List String) : Expr.toAst (Ast.toEx
 theorem Ast.macro_correct (a : Ast) : Expr.toAst (Ast.toExpr a []) [] = some a := toExpr_inv_toAst a []
 
 example := [stlc| λ x : ℕ . (λ y : ℕ → ℕ . free y x)]
+
+namespace Expr
+-- From I'm not a number I'm a free variable
+def abstract (expr : Expr) (target : FVarId) (idx : Nat := 0): Expr :=
+  match expr with
+  | .fvar name =>
+    if target = name then
+      .bvar idx
+    else
+      .fvar name
+  | .app fn arg => .app (abstract fn target idx) (abstract arg target idx )
+  | .lam ty body orig => .lam ty (abstract body target (idx + 1)) orig
+  | .const name => .const name
+  | .bvar idx => .bvar idx
+
+def instantiate (expr : Expr) (image : Expr) (targetIdx : Nat := 0) : Expr :=
+  match expr with
+  | .bvar idx =>
+    if idx = targetIdx then
+      image
+    else
+      .bvar idx
+  | .app fn arg => .app (instantiate fn image targetIdx ) (instantiate arg image targetIdx )
+  | .lam ty body orig => .lam ty (instantiate body image (targetIdx + 1)) orig
+  | .fvar name => .fvar name
+  | .const name => .const name
+
+inductive FVarIn (fvarId : FVarId) : Expr → Prop where
+| fvarEq : FVarIn fvarId (.fvar fvarId)
+| appLeft (func arg : Expr) (h : FVarIn fvarId func) : FVarIn fvarId (.app func arg)
+| appRight (func arg : Expr) (h : FVarIn fvarId arg) : FVarIn fvarId (.app func arg)
+| lam (ty : Ty) (body : Expr) (h : FVarIn fvarId body) : FVarIn fvarId (.lam ty body orig)
+
+def FreshIn (fvar : FVarId) (expr : Expr) := ¬ FVarIn fvar expr
+def Closed (expr : Expr) := ∀ fvar, FreshIn fvar expr
+
+inductive LocallyClosed : Expr → Prop where
+| const (name : String) : LocallyClosed (.const name)
+| fvar (fvarId : FVarId) : LocallyClosed (.fvar fvarId)
+| app (func arg : Expr) (closedFunc : LocallyClosed func) (closedArg : LocallyClosed arg) : LocallyClosed (.app func arg)
+| lam (ty : Ty) (body : Expr) (freeBody : FreshIn x body) (closedBody : LocallyClosed (abstract body x)) : LocallyClosed (.lam ty body orig)
+
+inductive ClosedTo : Nat → Expr → Prop where
+| const (n : Nat) (name : String) : ClosedTo n (.const name)
+| bvar (idx m : Nat) (closed : idx < m): ClosedTo m (.bvar idx)
+| fvar (n : Nat) (fvarId : FVarId) : ClosedTo n (.fvar fvarId)
+| app (func arg : Expr) (closedFunc : ClosedTo n func) (closedArg : ClosedTo n arg) : ClosedTo n (.app func arg)
+| lam (closedBody : ClosedTo (n + 1) body) : ClosedTo n (.lam ty body orig)
+
+abbrev LocallyClosed' (expr : Expr) := ClosedTo 0 expr
+
+abbrev _root_.Cube.WfExpr := { expr : Expr // LocallyClosed expr }
+
+theorem instantiate_abstract_self_eq (expr : Expr) (h : FreshIn target expr) : (expr.instantiate (.fvar target) i).abstract target i = expr := by
+  induction expr generalizing i with
+  | bvar =>
+    simp only [instantiate]
+    split <;> simp_all[abstract]
+  | fvar =>
+    simp only [instantiate, abstract]
+    split
+    next h2 =>
+      apply h
+      rw [h2]
+      apply FVarIn.fvarEq
+    next => rfl
+  | const => simp [abstract, instantiate]
+  | lam ty body orig bih =>
+    simp only [instantiate, abstract, lam.injEq, and_true, true_and]
+    apply bih
+    intro h2
+    apply h
+    apply FVarIn.lam
+    assumption
+  | app func arg fih aih =>
+    simp only [instantiate, abstract, app.injEq]
+    constructor
+    case left =>
+      apply fih
+      intro h2
+      apply h
+      apply FVarIn.appLeft
+      assumption
+    case right =>
+      apply aih
+      intro h2
+      apply h
+      apply FVarIn.appRight
+      assumption
+
+theorem abstract_instantiate_self_eq' (expr : Expr) (h : ClosedTo i expr) : (expr.abstract target i).instantiate (.fvar target) i = expr := by
+  induction expr generalizing i with
+  | bvar =>
+    simp only [instantiate, ite_eq_right_iff]
+    intro h2
+    cases h
+    linarith
+  | const => simp [abstract, instantiate]
+  | fvar =>
+    simp only [abstract]
+    split <;> simp_all [instantiate]
+  | app func arg fih aih =>
+    simp only [abstract, instantiate, app.injEq]
+    cases h
+    constructor
+    case left => apply fih; assumption
+    case right => apply aih; assumption
+  | lam ty body orig ihb =>
+    simp only [abstract, instantiate, lam.injEq, true_and, and_true] at *
+    cases h
+    apply ihb
+    assumption
+
+  
+theorem LocallyClosed'.succ_closed_of_abstract_closed (h : ClosedTo i (abstract expr x i)) : ClosedTo (i + 1) expr := by
+  induction expr generalizing i with
+  | bvar =>
+    simp only [abstract] at h
+    cases h
+    apply ClosedTo.bvar
+    linarith
+  | fvar => apply ClosedTo.fvar
+  | const => apply ClosedTo.const
+  | app func arg fih aih =>
+    cases h
+    apply ClosedTo.app
+    case closedFunc => apply fih; assumption
+    case closedArg => apply aih; assumption
+  | lam ty body tih bih =>
+    cases h
+    apply ClosedTo.lam
+    case closedBody => apply bih; assumption 
+
+theorem LocallyClosed.iff_LocallyClosed' (h : LocallyClosed expr) : LocallyClosed' expr := by
+  induction h with
+  | const => apply ClosedTo.const
+  | fvar => apply ClosedTo.fvar
+  | app =>
+    apply ClosedTo.app
+    repeat assumption
+  | lam =>
+    apply ClosedTo.lam
+    case closedBody =>
+      apply LocallyClosed'.succ_closed_of_abstract_closed
+      repeat assumption
+
+theorem abstract_instantiate_self_eq (expr : Expr) (h : LocallyClosed expr) : (expr.abstract target).instantiate (.fvar target) = expr := by
+  apply abstract_instantiate_self_eq'
+  apply LocallyClosed.iff_LocallyClosed'
+  assumption
+
+end Expr
 
 end Cube.Simple
 
