Cube/Simple/Typing.lean
@@ -2,82 +2,86 @@ import Cube.Context
 import Cube.Simple.Basic
 
 import Mathlib.Tactic.Linarith
+import Mathlib.Data.Finset.Basic
 
 namespace Cube.Simple
 
 namespace Expr
 
-inductive ClosedTo : Nat → Expr → Prop where
-| bvar (idx m : Nat) (closed : idx < m): ClosedTo m (.bvar idx)
-| lam (closed : ClosedTo (n + 1) body) : ClosedTo n (.lam ty body orig)
-| const (n : Nat) (name : String) : ClosedTo n (.const name)
-| app (func arg : Expr) (closedFunc : ClosedTo n func) (closedArg : ClosedTo n arg) : ClosedTo n (.app func arg)
-
-abbrev Closed (expr : Expr) := ClosedTo 0 expr
-
-def ClosedExpr := { expr : Expr // Closed expr }
-
 abbrev Context := Cube.Context Ty
-abbrev Env := String → Option Ty
+abbrev Env := Cube.Env Ty
 
 inductive Typing : Env → Context → Expr → Ty → Prop where
-| const (in_env : env name = some typ) : Typing env ctx (.const name) typ
-| app (func_type : Typing env ctx func (.fun t1 t2)) (arg_type : Typing env ctx arg t1) : Typing env ctx (.app func arg) t2
-| lam (body_type : Typing env (t1 :: ctx) body t2) : Typing env ctx (.lam t1 body orig) (.fun t1 t2)
-| bvar (idx : Nat) (bound : idx < ctx.length) : Typing env ctx (.bvar idx) (ctx.get ⟨idx, bound⟩)
+| const (name : String) (typ : Ty) (in_env : env.get name = some typ) : Typing env ctx (.const name) typ
+| fvar (fvarId : FVarId) (inContext : ctx.get fvarId = some ty) : Typing env ctx (.fvar fvarId) ty
+| app (func arg : Expr) (t1 t2 : Ty) (func_type : Typing env ctx func (.fun t1 t2)) (arg_type : Typing env ctx arg t1) : Typing env ctx (.app func arg) t2
+| lam ( body : Expr) (t1 t2 : Ty) (L : Finset FVarId) (body_type : ∀ fvarId , fvarId ∉ L → Typing env (ctx.update fvarId t1) (body.instantiate (.fvar fvarId)) t2) : Typing env ctx (.lam t1 body orig) (.fun t1 t2)
 
 notation:40 "("Δ ", " Γ ")" " ⊢ " e " : " t => Typing Δ Γ e t
 
-theorem ClosedTo.of_typed (h : (env, ctx) ⊢ expr : ty) : ClosedTo ctx.length expr := by
-  induction h with
-  | const => apply ClosedTo.const
-  | app _ _ func_ih arg_ih => simp [ClosedTo.app, *]
-  | bvar => simp [ClosedTo.bvar, *]
-  | lam =>
-    apply ClosedTo.lam
-    assumption
+/-
+TODO: Induction principle for empty context, this should allow easier arguing over closed terms
+TODO: Build machinery to fix the lam case
+TODO: Investigate cofinite quantification: https://www.chargueraud.org/research/2009/ln/main.pdf
+-/
+theorem LocallyClosed.of_typed (h : (env, Context.empty) ⊢ expr : ty) : LocallyClosed expr := by
+  cases h with
+  | const => apply LocallyClosed.const
+  | fvar fvarId ih => apply LocallyClosed.fvar
+  | app func arg t1 _ hfunc harg =>
+    have fih := of_typed hfunc
+    have aih := of_typed harg
+    apply LocallyClosed.app
+    repeat assumption
+  | lam body t1 t2 L hbody =>
+    apply LocallyClosed.lam
+    sorry
+    sorry
+    sorry
 
-def ClosedExpr.infer (expr : ClosedExpr) (env : Env) : Option Ty :=
-  go expr.val expr.property [] rfl
+def WfExpr.infer (expr : WfExpr) (env : Env) : Option Ty :=
+  go expr.val expr.property Context.empty
 where
-  go {n : Nat} (expr : Expr) (h1 : ClosedTo n expr) (ctx : Context) (h2 : ctx.length = n) : Option Ty :=
+  go (expr : Expr) (h1 : LocallyClosed expr) (ctx : Context) : Option Ty :=
     match expr with
-    | .bvar idx =>
-      if hVar:idx < n then
-        some <| ctx.get ⟨idx, h2 ▸ hVar⟩
-      else
-        none
+    | .bvar .. => none
     | .app fn arg => Id.run do
-      have closedFn : ClosedTo n fn := by
+      have closedFn : LocallyClosed fn := by
         cases h1; assumption
-      have closedArg : ClosedTo n arg := by
+      have closedArg : LocallyClosed arg := by
         cases h1; assumption
-      if let some (.fun t1 t2) := go fn closedFn ctx h2 then
-        if let some t3 := go arg closedArg ctx h2 then
+      if let some (.fun t1 t2) := go fn closedFn ctx then
+        if let some t3 := go arg closedArg ctx then
           if t1 = t3 then
             return some t2
       return none
-    | .lam t1 body _ =>
-      have bodyClosed : ClosedTo (ctx.length + 1) body := by
+    | .lam t1 body orig =>
+      let newFVar := FVar.fresh ctx
+      let newCtx := ctx.update newFVar t1
+      let newBody := body.instantiate (.fvar newFVar)
+      have bodyClosed : LocallyClosed newBody := by
         cases h1
-        rw [h2]
-        assumption
-      if let some t2 := go body bodyClosed (t1 :: ctx) rfl then
+        sorry
+      -- TODO: Instantiate .fvar preserves size
+      -- Note: sizeOf for Expr looks at the content of data, I don't want that, .fvar and .bvar should always have size 1
+      -- -> I'll need a custom size measure to make this pretty
+      have wf : sizeOf (instantiate body (fvar (FVar.fresh ctx))) < 1 + sizeOf t1 + sizeOf body + sizeOf orig := sorry
+      if let some t2 := go newBody bodyClosed newCtx then
         some (.fun t1 t2)
       else
         none
-    | .fvar .. => nomatch h1
-    | .const name =>
-      match env name with
-      | some ty => some ty
-      | none => none
+    | .fvar fvarId => ctx.get fvarId
+    | .const name => env.get name 
+termination_by go expr h1 ctx => expr
 
-theorem ClosedExpr.infer.go_sound (expr : Expr) (env : Env) (ctx : Context) (h1 : ClosedTo ctx.length expr) (h2 : ClosedExpr.infer.go env expr h1 ctx rfl = some t) : (env, ctx) ⊢ expr : t := by
+theorem WfExpr.infer.go_sound (expr : Expr) (env : Env) (ctx : Context) (h1 : LocallyClosed expr) (h2 : WfExpr.infer.go env expr h1 ctx = some t) : (env, ctx) ⊢ expr : t := by
   induction expr generalizing t ctx with
-  | fvar => contradiction
+  | bvar => contradiction
+  | fvar => sorry
   | const name =>
     unfold infer.go at h2
-    split at h2 <;> simp [Typing.const, *]
+    apply Typing.const
+    assumption
   | app f x fih xih =>
     simp only [infer.go, Id.run] at h2
     repeat split at h2
@@ -99,15 +103,11 @@ theorem ClosedExpr.infer.go_sound (expr : Expr) (env : Env) (ctx : Context) (h1 
       injections h2
       rw[←h2]
       apply Typing.lam
-      apply ih
-      exact h3
+      case L => sorry
+      case body_type =>
+        intro fvarId hf
+        sorry
     next => contradiction
-  | bvar idx =>
-    have idx_get : t = ctx.get ⟨idx, (by cases h1; assumption)⟩ := by
-      unfold go at h2
-      split at h2 <;> simp_all
-    rw[idx_get]
-    apply Typing.bvar
 
 theorem ClosedExpr.infer_sound (expr : ClosedExpr) (env : Env) (h : expr.infer env = some t) : (env, []) ⊢ expr.val : t := by
   unfold infer at h
@@ -202,34 +202,6 @@ theorem Typing.weakening (h1 : ctx' = ctx ++ additional) (h2 : (env, ctx) ⊢ ex
 
 theorem Typing.weakening_empty (ctx : Context) (h : (env, []) ⊢ expr : typ) : (env, ctx) ⊢ expr : typ :=
   Typing.weakening (List.nil_append ctx).symm h
-
--- From I'm not a number I'm a free variable
-def abstract (target : String) (expr : Expr) (idx : Nat := 0): Expr :=
-  match expr with
-  | .fvar name =>
-    if target = name then
-      .bvar idx
-    else
-      .fvar name
-  | .app fn arg => .app (abstract target fn idx) (abstract target arg idx )
-  | .lam ty body orig => .lam ty (abstract target body (idx + 1)) orig
-  | .const name => .const name
-  | .bvar idx => .bvar idx
-
-def instantiate (image : Expr) (expr : Expr) (targetIdx : Nat := 0): Expr :=
-  match expr with
-  | .bvar idx =>
-    if idx = targetIdx then
-      image
-    else
-      .bvar idx
-  | .app fn arg => .app (instantiate image fn targetIdx ) (instantiate image arg targetIdx )
-  | .lam ty body orig => .lam ty (instantiate image body (targetIdx + 1)) orig
-  | .fvar name => .fvar name
-  | .const name => .const name
-
-def substitute (image : Expr) (name : String) (expr : Expr) : Expr :=
-  expr.abstract name |>.instantiate image
 
 theorem Typing.instantiate_preserves (h1 : (env, []) ⊢ v : ty) (h2 : (env, (Context.set ctx i ty)) ⊢ expr : ty') : (env, ctx) ⊢ (instantiate v expr i) : ty' := by
   induction expr generalizing ctx ty' i with
